src/computational_monads/simulation_semantics/oracle_compose.lean
@@ -2,25 +2,24 @@ import computational_monads.simulation_semantics.default_simulate
 
 open oracle_comp oracle_spec
 
-variables {spec spec' spec'' : oracle_spec} {A B C : Type}
+variables {spec spec' spec'' : oracle_spec} {A B C : Type} {S S' : Type}
 
 namespace simulation_oracle
 
-def oracle_compose (so : simulation_oracle spec spec') (so' : simulation_oracle spec' spec'') :
-  simulation_oracle spec spec'' :=
-{ S := so.S × so'.S,
-  default_state := (so.default_state, so'.default_state),
+def oracle_compose (so : simulation_oracle spec spec' S)
+  (so' : simulation_oracle spec' spec'' S') : simulation_oracle spec spec'' (S × S') :=
+{ default_state := (so.default_state, so'.default_state),
   o := λ i x, simulate so' (so i (x.1, x.2.1)) x.2.2 >>= λ u_s, pure (u_s.1.1, u_s.1.2, u_s.2) }
 
 notation so' `∘ₛ` so := oracle_compose so so'
 
-variables (so : simulation_oracle spec spec') (so' : simulation_oracle spec' spec'')
+variables (so : simulation_oracle spec spec' S) (so' : simulation_oracle spec' spec'' S')
 
 @[simp]
 lemma default_state_oracle_compose :
   (so' ∘ₛ so).default_state = (so.default_state, so'.default_state) := rfl
 
-lemma oracle_compose_apply_index (i : spec.ι) (s : so.S × so'.S) : (so' ∘ₛ so) i =
+lemma oracle_compose_apply_index (i : spec.ι) (s : S × S') : (so' ∘ₛ so) i =
   λ x, simulate so' (so i (x.1, x.2.1)) x.2.2 >>= λ u_s, pure (u_s.1.1, u_s.1.2, u_s.2) := rfl
 
 section support
