src/computational_monads/simulation_semantics/constructions/counting_oracle.lean
@@ -15,7 +15,7 @@ variables {α β γ : Type} {spec spec' : oracle_spec}
   (oa : oracle_comp spec α) (ob : α → oracle_comp spec β) (n m : ℕ)
 
 /-- Simulation oracle that just counts the number of queries to the oracles -/
-def counting_oracle (spec : oracle_spec) : simulation_oracle spec spec :=
+def counting_oracle (spec : oracle_spec) : simulation_oracle spec spec ℕ :=
 ⟪query | λ n _ _ _, n + 1 , 0⟫
 
 namespace counting_oracle
@@ -26,9 +26,11 @@ tracking_oracle.apply_eq query (λ n _ _ _, n + 1) 0 i x
 
 section support
 
+@[simp]
 lemma support_apply (i : spec.ι) (x : spec.domain i × ℕ) :
   (counting_oracle spec i x).support = {y | y.2 = nat.succ x.2} :=
-(tracking_oracle.support_apply query _ _ i x).trans (by simpa)
+(tracking_oracle.support_apply query _ _ i x).trans
+  (by simp only [support_query, set.top_eq_univ, set.mem_univ, true_and])
 
 end support
 
