src/computational_monads/simulation_semantics/constructions/logging/caching_oracle.lean
@@ -7,9 +7,8 @@ open oracle_comp oracle_spec
 variables {A B C : Type} {spec spec' spec'' : oracle_spec}
 
 def caching_oracle (spec : oracle_spec) [spec.computable] :
-  simulation_oracle spec spec :=
-{ S := query_log spec,
-  default_state := query_log.init spec,
+  simulation_oracle spec spec (query_log spec) :=
+{ default_state := query_log.init spec,
   o := λ i ⟨t, log⟩, match log.lookup i t with
   | (some u) := return (u, log) -- Return the cached value if it already exists
   | none := do { u ← query i t, return (u, log.log_query i t u) }
