src/computational_monads/simulation_semantics/constructions/logging/seeded_oracle.lean
@@ -25,9 +25,8 @@ variables {spec spec' spec'' : oracle_spec} {A B C : Type}
   If the query values don't match then throw away the seed as computation has diverged.
   Using this with a log from a previous computation ensures they behave identically. -/
 def seeded_oracle (spec : oracle_spec) [computable spec] :
-  simulation_oracle spec spec :=
-{ S := query_log spec,
-  default_state := query_log.init spec,
+  simulation_oracle spec spec (query_log spec) :=
+{ default_state := query_log.init spec,
   o := λ i ⟨t, seed⟩, match seed.lookup_fst i t with
     -- Once the seed is empty, just keep it empty going forward
     | none := (λ u, (u, query_log.init spec)) <$> query i t
