src/computational_monads/simulation_semantics/constructions/uniform_oracle.lean
@@ -6,15 +6,13 @@ open oracle_comp oracle_spec
 variables {A B : Type} {spec spec' spec'' : oracle_spec}
 
 noncomputable def uniform_oracle (spec : oracle_spec) [spec.finite_range] : 
-  simulation_oracle spec uniform_selecting :=
+  simulation_oracle spec uniform_selecting unit :=
 ⟪λ i t, $ᵗ (spec.range i)⟫
 
 namespace uniform_oracle
 
 variables (oa : oracle_comp spec A)
 variable [spec.finite_range]
-
-noncomputable instance S_unique : unique (uniform_oracle spec).S := stateless_oracle.S_unique _
 
 @[simp]
 lemma apply_eq (i : spec.ι) (t : spec.domain i) (u : unit) :
@@ -27,10 +25,7 @@ by simp only [set.eq_univ_iff_forall, apply_eq, support_bind, support_uniform_se
   set.top_eq_univ, support_pure, set.Union_true, set.Union_singleton_eq_range, set.mem_range,
   prod.forall, prod.mk.inj_iff, exists_eq_left, forall_const, eq_iff_true_of_subsingleton]
 
-
-
 section eval_dist
-
 
 end eval_dist
 
